theories/IL/InRel.v
@@ -1,4 +1,4 @@
-Require Import Util LengthEq AllInRel Map Env IL AutoIndTac MoreList.
+Require Import Util EqDec LengthEq AllInRel Map Env IL AutoIndTac MoreList.
 Require Export DecSolve BlockType.
 
 Set Implicit Arguments.
